README.md
@@ -1,66 +1,11 @@
-# ArchSem
+# Operational/axiomatic sequential refinement proof
+# THIS IS AN OLD, FORKED VERSION OF ARCHSEM ONLY USED FOR THIS VERY SPECIFIC PROOF
 
-ArchSem is a Rocq framework to define the semantics of CPU architectures
-such as Arm-A, RISC-V, and x86, integrating their concurrency and instruction-set semantics.
-The framework is designed to be generic, but so far is only instantiated for Arm-A and RISC-V.
+**For the actual, up-to-date ArchSem refer to the main supplemented archive.**
+This development should only be used to inspect the proof that the operational
+sequential model refines the SC axiomatic model.
 
-
-## General goals and organization
-
-In order to build an architecture model one needs two components:
-- An _ISA model_ that provides the semantics of instructions. Those are intended
-  to be derived from [Sail](https://github.com/rems-project/sail) or
-  [ASL](https://developer.arm.com/Architectures/Architecture%20Specification%20Language)
-  specifications such as [sail-arm](https://github.com/rems-project/sail-arm) (via Sail).
-  We are currently working on a path to extract those from Sail, which is not
-  fully operational yet.
-- A _concurrency model_ that defines how the instructions interact with each
-  other, both in the same thread and between threads.  In other words, a
-  concurrency model is the missing part that take one from an ISA model to a
-  full architecture model. It is generally much smaller but much
-  more intricate than the instruction semantics. It contains both simple details like piping registers from
-  one instruction to the next all the way up to user relaxed-concurrency models and 
-  system-level concurrency models that have features such as instruction
-  fetching, virtual memory and architectural exceptions. Those concurrency
-  models will be written directly in Rocq for the immediate future, although
-  we plan ways to import the relaxed memory parts from existing relaxed
-  memory tools such as [Herd](https://github.com/herd/herdtools7) or
-  [Isla Axiomatic](https://github.com/rems-project/isla).
-
-ArchSem defines an [_Interface_](ArchSem/Interface.v) between the two so
-that they can interoperate properly. It is based on free monads (which are finite
-itrees, because the semantics of a single instruction cannot diverge). The interface is
-therefore mainly defined by the set of effects an instruction can call. This is
-mostly generic but allows precise architecture-specific customization points.
-This interface is derived from the Sail "outcomes" used by concurrency-aware
-Sail specifications. This allows one to plug an arbitrary ISA model with an arbitrary
-concurrency model and obtain an architecture model. It also allows making
-proofs about concurrency model against an arbitrary universally quantified ISA
-model and vice versa.
-
-More generally what want to enable with this framework includes:
-- Proving properties of CPU architectures
-- Proving correctness of software running on an architecture, especially system
-  software, in particular with the use of higher-level program logics, often
-  built using [Iris](https://iris-project.org/)
-- Proving correctness of compilers or compiler passes targeting the
-  architecture, including concurrency aspects
-- Proving equivalences and refinements between different models
-- Executing models on simple litmus tests to evaluate them and compare them to
-  other executable models
-- As a design tool to support thinking about architecture models for new features
-
-This places some constraints on how the framework can work, and in particular on
-the interface between ISA and concurrency models:
-- Things must as executable as possible. Our interface requires ISA model to be
-  executable, therefore if a concurrency model is made to be executable, the
-  resulting combination is executable. However, we haven't yet finished the
-  extraction pipeline and utilities to parse litmus tests to run.
-- The interface must support all kinds of concurrency models: axiomatic,
-  micro-architectural operations, promising, etc.
-- All models can be partial, so the framework must handle partiality properly.
-  ISA models can fail at any point and those failures must be correctly propagated
-  upwards. 
+The proof can be found in [ArchSemArm/CDestruct.v](ArchSemArm/ArmSeqAxOpEq.v).
 
 ## Building
 
@@ -73,32 +18,7 @@ There are some powerful custom tactics in `Common`, as well as useful but
 generic library. See the [README](Common/README.md) there for more details. In
 particular `cdestruct` is in [Common/CDestruct.v](Common/CDestruct.v).
 
-## The current state and directory structure
 
-- `Common` (Rocq module name `ASCommon`) is the "utils" library. It contains all
-  non-ArchSem-specific Rocq lemmas and automation, as well as required theories
-  such that executable relational algebra or effects and free monads.
-  This includes:
-  - `CDestruct.v` The implementation of the `cdestruct` tactic
-- `ArchSem` The architecture generic part of the projects, this includes
-  - `Interface.v` The definition of the interface between ISA models and
-    concurency models
-  - `CandidateExecution.v` The definition of candidate executions for weak
-    memory model
-- `ArchSemArm` The Armv9-A instantiation of the library. This includes
-  - A sequential operational model (`ArmSeqModel.v`)
-  - A User-mode promising model (`UMPromising.v`), similar to 
-    [the PLDI19 paper](https://sf.snu.ac.kr/publications/promising-arm-riscv.pdf)
-  - A very WIP VMSA promising model (`VMPromising.v`)
-  - A User-mode axiomatic model (`UMArm.v`)
-  - An SC model for Arm (`UMSeqArm.v`) that is unsound for >1 thread
-  - The VMSA model from [the ESOP22
-  paper](https://www.cl.cam.ac.uk/~pes20/iflat/top-extended.pdf) (`VMSA22Arm.v`)
-- `ArchSemRiscV` The RISC-V instantiation of the library. This is barebones for
-  now, but will be improved upon later
-- `Extraction` contains machinery to extract the code to OCaml, for now it is
-  mainly use to check that the code _can_ be extracted rather than as an
-  actually usable OCaml library
 
 ## Documentation
 
@@ -108,44 +28,3 @@ will be generated in:
 - `_build/default/Common/ASCommon.html/toc.html`
 - `_build/default/ArchSem/ArchSem.html/toc.html`
 - `_build/default/ArchSemArm/ArchSemArm.html/toc.html`
-- `_build/default/ArchSemRiscV/ArchSemRiscV.html/toc.html`
-
-
-## Current limitations
-
-Developing complete architectural models is an ambitious long-term goal. The
-curent state takes many important steps towards that, but there is still much to
-do. In the short term, this includes:
-
-### Connection to Sail
-
-We have almost all of the pipeline to import a Sail model into ArchSem done, but
-some details remain.
-
-### Test runner
-
-While most of the code can run in Rocq we currently do not have a good working
-extraction pipeline, or a CLI frontend to call models on litmus
-tests. 
-
-### Partiality handling
-
-In order to allow partial models and execution traces that contain partially
-executed instructions, we need more support from the interface to bound what a
-partially executed instruction can do next. Concurrency models must therefore correctly
-understand this information to handle undefined behaviour properly.
-
-### Intra-instruction parallelism
-
-Currently, the interface and instruction semantics is based on the instruction
-semantics being a free monad, which totally orders all the effects that an
-instruction can emit. We need to relax that constraint to allow instructions to
-emit multiple effects in parallel. This cannot be achieved with
-non-deterministic interleaving because of intricate details on relaxed
-architectures like Arm.
-
-## Git history
-
-Commits before 2024-12-19 were extracted with `git filter-repo` from a private
-repository and were kept for `git blame` but might not build except for the most
-recent ones.
